---
title: Notes on M. Kimura 1964 (2)
categories:
- "Population Genetics"
comments: true
feature_image: "https://picsum.photos/2560/600?image=872"
---

Using the notations above, the proof of (3.2) easily follows from the definition of continuous stochastic process.
\begin{align}
    \int_{|\delta x| \geq \epsilon} g(\delta x,x; \delta t, t) d(\delta x) 
    &= \mathbf{P} \( |Y_{\delta t, t}| \geq \epsilon |X_t=x\) \newline
    &\leq \frac{\mathbf{P} \( |X_{t+\delta t}-X_t| \geq \epsilon \)}{\mathbf{P}(X_t=x)} \newline
    &= o(\delta t)
\end{align}

The next equation (3.3) can be proved using simple rules of integration.
We have defined $Y_{\delta t,t} = X_{t+\delta t}-X_t$.
\begin{align}
    \mathbf{P}(X_{t+\delta t} \in [a,b]) &= \mathbf{P}(Y_{\delta t,t}+X_t \in [a,b]) \newline
          &= \mathbf{P}((X_t, Y_{\delta t,t}) \in U)
\end{align}
where $U=\\{(x,y) \in \mathbb{R}^2:x+y \in [a,b] \\}$.

Let $f_{X_t, Y_{\delta t,t}}$ be the joint density.
Then the above equation becomes
\begin{align}
    \int_{U} f_{X_t, Y_{\delta t,t}}(x,y) dxdy &= \int_{U} f_{X_t}(x)f_{Y_{\delta t,t}|X_{t}}(y|x)dxdy \newline
    &= \int_{U} \phi(p,x;t)g(y,x;\delta t, t) dydx \newline
    &= \int_{[a,b]} \int_{\mathbb{R}} \phi(p,x'-y';t)g(y',x'-y';\delta t, t) dy'dx'
\end{align}
Change of variables theorem was used with $T(x,y)=(x',y')$ where 
$T=\begin{pmatrix} 1 & 1 \newline 0 & 1 \end{pmatrix}$.

Therefore, by the uniqueness of density, we have
\begin{align}
\phi(p,x;t+\delta t) = \int_{\mathbb{R}} \phi(p,x-y;t)g(y,x-y;\delta t, t) dy
\end{align}

